stable proofs of both translation theorems

Tree_calculus/Abstraction.v
@@ -58,11 +58,57 @@ Qed.
   
 
 
-Lemma h_fn_not_omega: h_fn <> omega_k 3. 
-Proof. unfold h_fn, omega_k; intro H; discriminate. Qed. 
+Lemma h_fn_not_omega: forall k, h_fn <> omega_k k. 
+Proof.
+  intros. 
+  unfold omega_k.
+  rewrite star_opt_occurs_true.
+  2: unfold app_comb; unfold_op; unfold occurs, eqnat, plus. 
+  2: rewrite occurs_closed; auto. 2: discriminate.
+  unfold star_opt at 3.
+  unfold app_comb at 1.
+  rewrite (star_opt_occurs_true (App (Op Node) (App (Op Node) i_op))).
+  2: rewrite ! occurs_app. 
+  2: replace (occurs 0 (Ref 0)) with 1 by (cbv; auto); omega.
+  2: discriminate.
+  rewrite (star_opt_closed (App (Op Node) (App (Op Node) i_op))). 
+  2: cbv; auto. 
+  rewrite (star_opt_occurs_true (App (Op Node) (App (Op Node) (App k_op (Ref 0))))).
+  2: rewrite ! occurs_app. 
+  2: replace (occurs 0 (Ref 0)) with 1 by (cbv; auto); omega.
+  2: discriminate.
+  rewrite (star_opt_occurs_true (Op Node)). 
+  2: cbv; auto. 
+  2: discriminate.
+  rewrite (star_opt_occurs_true (Op Node)). 
+  2: cbv; auto. 
+  2: discriminate.
+  rewrite (star_opt_eta k_op). 
+  2: cbv; auto. 
+  rewrite (star_opt_closed (Op Node)); auto. subst_tac.
+  rewrite (star_opt_occurs_false (App (App (Op Node) (Op Node))
+                                      (app_comb (app_comb (A_k (S k)) (Ref 1)) (Ref 1)))).
+  2: unfold app_comb; rewrite ! occurs_app.
+  2: rewrite (occurs_closed 0 (A_k (S k))).
+  2: cbv; auto.   
+  2: rewrite A_k_closed; auto.   subst_tac.
+  rewrite ! subst_rec_preserves_app_comb.
+  rewrite subst_rec_closed.
+  2: rewrite A_k_closed; auto. subst_tac. 
+  rewrite star_opt_occurs_true. 
+  2: unfold app_comb; unfold_op; rewrite ! occurs_app. 
+  2: rewrite (occurs_closed 0 (A_k _)).  2: cbv;auto. 2: apply A_k_closed.
+  2: discriminate.
+  unfold h_fn.
+  unfold star_opt at 4. unfold occurs, eqnat, plus. subst_tac. 
+  unfold star_opt at 3. unfold occurs, eqnat, plus. subst_tac. 
+  unfold star_opt at 2. unfold occurs, eqnat, plus. subst_tac. 
+  unfold star_opt at 1. unfold occurs, eqnat, plus. subst_tac. 
+  discriminate.
+Qed. 
 
  
-Definition h_op := app_comb (Y_k 4) h_fn .
+Definition h_op := app_comb (Y_k 2) h_fn .
 
 Lemma h_red: forall M N P, sf_red (App (App (App h_op M) N) P) (App (App h_op (App (App h_op M) N)) P).
 Proof.
@@ -70,7 +116,7 @@ intros. unfold h_op at 1.
 eapply transitive_red.
 eapply preserves_app_sf_red. eapply preserves_app_sf_red. eapply2 app_comb_red. all: auto. 
 eapply transitive_red.    
-eapply2 Y4_fix.
+eapply2 Y2_fix.
 unfold h_fn at 1. 
 eapply transitive_red.
 eapply preserves_app_sf_red. 
@@ -97,24 +143,24 @@ Qed.
 
   
   
-Definition j_op := app_comb (Y_k 2) h_op. 
+Definition j_op := app_comb (Y_k 0) h_op. 
 
 Lemma j_red: forall M, sf_red (App j_op M) (App (App h_op j_op) M).
 Proof. 
 intros. unfold j_op at 1. 
 eapply transitive_red. eapply2 app_comb_red. 
-eapply transitive_red. eapply2 Y2_fix. 
+eapply transitive_red. eapply2 Y0_fix. 
 eapply2 zero_red. 
 Qed. 
 
 
-Definition r_op := app_comb (Y_k 3) (app_comb compose h_op).
+Definition r_op := app_comb (Y_k 1) (app_comb compose h_op).
 
 Lemma r_red : forall M N, sf_red (App (App r_op M) N) (App (App h_op (App r_op M)) N).
 Proof. 
 intros. unfold r_op at 1. 
 eapply transitive_red. eapply preserves_app_sf_red. eapply2 app_comb_red. auto.  
-eapply transitive_red. eapply2 Y3_fix. 
+eapply transitive_red. eapply2 Y1_fix. 
 eapply transitive_red. eapply preserves_app_sf_red. eapply preserves_app_sf_red.  
 eapply2 app_comb_red. all: auto.  
 eapply transitive_red. eapply preserves_app_sf_red. eapply2 compose_composes. auto. 
@@ -122,7 +168,7 @@ eapply transitive_red. eapply preserves_app_sf_red. eapply2 compose_composes. au
 Qed. 
 
 Lemma r_aux: 
-forall M N , sf_red (App (App (Y_k 3) M) N) (app_comb (app_comb (app_comb (omega_k 3) (omega_k 3)) M) N) . 
+forall M N , sf_red (App (App (Y_k 1) M) N) (app_comb (app_comb (app_comb (omega_k 1) (omega_k 1)) M) N) . 
 Proof. 
 intros; unfold Y_k.
 eapply transitive_red. eapply preserves_app_sf_red.
@@ -148,17 +194,17 @@ Definition ab_fn b' :=
   star_opt (star_opt (star_opt (App (App (App b' (Ref 0)) (Ref 2)) (Ref 1)))). 
 (* b' is presumed closed *)
 Definition ab_op ab' := 
-star_opt (star_opt (app_comb2 (app_comb (app_comb (A_k 3) ab') (Ref 1)) (Ref 0))).
+star_opt (star_opt (app_comb2 (app_comb (app_comb (A_k 1) ab') (Ref 1)) (Ref 0))).
 
 Lemma a_aux: forall b' M N, maxvar b' = 0 -> sf_red (App (App (ab_op (ab_fn b')) M) N) 
- (app_comb2 (app_comb (app_comb (A_k 3) (ab_fn b')) M) N).
+ (app_comb2 (app_comb (app_comb (A_k 1) (ab_fn b')) M) N).
 Proof. 
 intros. 
 eapply transitive_red.
 unfold ab_op. eapply2 star_opt_beta2.
 unfold subst; rewrite ! subst_rec_preserves_app_comb2.
 rewrite ! subst_rec_preserves_app_comb.
-rewrite ! (subst_rec_closed (A_k 3)).
+rewrite ! (subst_rec_closed (A_k 1)).
 2: rewrite A_k_closed; omega.
 rewrite ! (subst_rec_closed (ab_fn b')).
 all: cycle 1. 
@@ -231,7 +277,7 @@ Definition ab1 b' P :=
                                                (App (App (Op Node) (Op Node))
                                                   b')))
                                          (App (App (Op Node) (Op Node))
-                                            (A_k 3))))))))))))))
+                                            (A_k 1))))))))))))))
      (star_opt
         (App (Op Node)
            (App (Op Node)
@@ -257,63 +303,81 @@ unfold app_comb at 1.
 rewrite star_opt_occurs_true.
 all: cycle 1. 
 rewrite ! occurs_app. 
-replace (occurs 0 (Ref 0)) with true by auto. 
-rewrite orb_true_r at 1. 
-rewrite orb_true_r at 1. 
-rewrite orb_true_r at 1. 
-rewrite orb_true_r at 1. 
-rewrite orb_true_r at 1. 
-auto. 
+replace (occurs 0 (Ref 0)) with 1 by auto. 
+omega. 
 discriminate. 
 rewrite star_opt_occurs_true.
 all: cycle 1. 
 rewrite ! occurs_app. 
-replace (occurs 0 (Ref 0)) with true by auto. 
-rewrite orb_true_r at 1. 
-rewrite orb_true_r at 1. 
-rewrite orb_true_r at 1. 
-rewrite orb_true_r at 1. 
-auto. 
+replace (occurs 0 (Ref 0)) with 1 by auto.
+omega.
 discriminate.
-unfold_op; unfold star_opt at 1. 
-unfold occurs. 
-rewrite ! orb_false_l.
-unfold eqnat. 
-rewrite orb_true_l. 
-repeat eapply2 preserves_app_sf_red. 
-(* 1 *) 
-rewrite star_opt_occurs_false.
+rewrite star_opt_occurs_true.
 all: cycle 1. 
-rewrite ! occurs_app.
-rewrite ! occurs_op. 
-rewrite occurs0_lift. 
-rewrite occurs_closed. auto. auto. 
-(* 1 *) 
-simpl. 
-repeat eapply2 preserves_app_sf_red. 
-(* 1 *) 
-unfold lift; rewrite subst_rec_lift_rec; try omega.
-rewrite lift_rec_null; auto.
-rewrite subst_rec_closed. 2: rewrite H; omega. 
-auto. 
+rewrite ! occurs_app. 
+replace (occurs 0 (Ref 0)) with 1 by auto.
+omega.
+discriminate.
+rewrite star_opt_occurs_true.
+all: cycle 1. 
+rewrite ! occurs_app. 
+replace (occurs 0 (Ref 0)) with 1 by auto.
+omega.
+discriminate.
+rewrite star_opt_closed. 2: cbv; auto. 
+rewrite star_opt_occurs_true.
+all: cycle 1. 
+rewrite ! occurs_app. 
+replace (occurs 0 (Ref 0)) with 1 by auto.
+omega.
+discriminate.
+rewrite star_opt_occurs_true.
+all: cycle 1. 
+rewrite ! occurs_app. 
+replace (occurs 0 (Ref 0)) with 1 by auto.
+omega.
+discriminate.
+rewrite star_opt_eta. 2: cbv; auto.
+rewrite (star_opt_occurs_false (App (Op Node)
+                      (App (Op Node)
+                           (App k_op (app_comb (app_comb (A_k 1) b') (lift 1 P)))))).
+2: unfold_op; simpl. 2: unfold lift; rewrite occurs_lift_rec_zero.
+2: rewrite occurs_closed; auto. subst_tac.
+rewrite ! star_opt_closed. subst_tac.
+all: cycle 1.
+cbv; auto.
+cbv; auto.
+auto.
+(* 1 *)
+subst_tac. rewrite ! subst_rec_preserves_app_comb.
+rewrite subst_rec_closed.
+2: rewrite A_k_closed; auto.
+rewrite subst_rec_closed.
+2: rewrite H; auto.
+unfold lift;  subst_tac.
+unfold ab1.
+rewrite star_opt_closed.
+2: cbv; auto.
+unfold app_comb; unfold_op.  
+apply zero_red.
 Qed. 
 
 
 
 Definition b_fn := 
 star_opt (star_opt (star_opt (
-extension (app_comb (app_comb (app_comb (app_comb (omega_k 4) (omega_k 4)) h_fn) (Ref 0)) (Ref 1))
+extension (app_comb (app_comb (app_comb (app_comb (omega_k 2) (omega_k 2)) h_fn) (Ref 0)) (Ref 1))
           (App (App (App (App (Ref 4) (Ref 3)) (Ref 2)) (Ref 0))   (* H (Ref 0) (Ref 1) *)
                (App (App (App (Ref 4) (Ref 3)) (Ref 2)) (Ref 1))) (
-extension (app_comb (app_comb (app_comb (app_comb (omega_k 4) (omega_k 4)) (Ref 0)) (Ref 1)) (Ref 2)) (
-          (App (App (app_comb (app_comb (app_comb (A_k 5) (omega_k 4)) (omega_k 4)) (Ref 0))
+extension (app_comb (app_comb (app_comb (app_comb (omega_k 2) (omega_k 2)) (Ref 0)) (Ref 1)) (Ref 2)) (
+          (App (App (app_comb (app_comb (app_comb (A_k 3) (omega_k 2)) (omega_k 2)) (Ref 0))
                (App (App (App (Ref 5) (Ref 4)) (Ref 3)) (Ref 1)))   (* B (Ref 0) (Ref 1) *)
                (App (App (App (Ref 5) (Ref 4)) (Ref 3)) (Ref 2))) ) (
-extension (app_comb (app_comb (app_comb (omega_k 3) (omega_k 3)) (Ref 0)) (Ref 1)) (* R (Ref 1) *) 
+extension (app_comb (app_comb (app_comb (omega_k 1) (omega_k 1)) (Ref 0)) (Ref 1)) (* R (Ref 1) *) 
           (App (Ref 2) (Ref 1)) (
-extension (app_comb (Y_k 2) (Ref 0)) (* J *) 
+extension (app_comb (Y_k 0) (Ref 0)) (* J *) 
           (Ref 2)  ( 
-extension (app_comb2 (app_comb (app_comb (A_k 3) (Ref 0)) (Ref 1)) (Ref 2))  (* A B' (Ref 1) (Ref 2) *) 
+extension (app_comb2 (app_comb (app_comb (A_k 1) (Ref 0)) (Ref 1)) (Ref 2))  (* A B' (Ref 1) (Ref 2) *) 
                                        (* use (Ref 3) not (Ref 1) because ab_op binds two times *) 
           (App (App (ab_op (Ref 3))
                     (App (App (App (Ref 5) (Ref 4)) (Ref 3)) (Ref 2))) 
@@ -323,11 +387,11 @@ extension (ab1 (Ref 0) (Ref 1))
           (App (App (App (App (Ref 4) (Ref 3)) (Ref 2)) (ab_op (Ref 2)))
                (App (App (App (Ref 4) (Ref 3)) (Ref 2)) (Ref 1))) (
                                        (* use (Ref 2) not (Ref 0) because ab_op binds two times *) 
-extension (app_comb a_op (app_comb (app_comb (app_comb (omega_k 4) (omega_k 4)) (Ref 0)) (Ref 1)))
+extension (app_comb a_op (app_comb (app_comb (app_comb (omega_k 2) (omega_k 2)) (Ref 0)) (Ref 1)))
           (App 
 
 (App (App (App (Ref 4) (Ref 3)) (Ref 2)) 
-(app_comb (app_comb (app_comb (A_k 5) (omega_k 4)) (omega_k 4)) (Ref 0)))
+(app_comb (app_comb (app_comb (A_k 3) (omega_k 2)) (omega_k 2)) (Ref 0)))
 
 (App (App (App (Ref 4) (Ref 3)) (Ref 2)) 
  (Ref 1)))
@@ -336,18 +400,11 @@ i_op)))))))))
 .
 
 
-Definition b_op := app_comb (Y_k 4) b_fn .
+Definition b_op := app_comb (Y_k 2) b_fn .
 
 Definition abs_op := ab_op (ab_fn b_op). 
 
  
-
-Lemma pattern_size_app_comb2 : 
-forall M N, pattern_size (app_comb2 M N) = pattern_size M + pattern_size N. 
-Proof. 
-intros. unfold app_comb2. rewrite pattern_size_app_comb. 
-unfold flip. unfold_op. simpl. omega. 
-Qed. 
 
 Lemma maxvar_ab_fn: forall M, maxvar (ab_fn M) = pred (pred (pred (maxvar M))). 
 Proof. 
@@ -381,6 +438,15 @@ Qed.
 Lemma pattern_size_ab1: forall b' P, pattern_size (ab1 b' P) = pattern_size P + pattern_size b'.
 Proof.
 intros. cbv. fold plus. rewrite ! plus_0_r. auto.  
+Qed. 
+
+
+
+Lemma pattern_size_app_comb2 : 
+forall M N, pattern_size (app_comb2 M N) = pattern_size M + pattern_size N. 
+Proof. 
+intros. unfold app_comb2. rewrite pattern_size_app_comb. 
+unfold flip. unfold_op. simpl. omega. 
 Qed. 
 
 
@@ -419,7 +485,7 @@ Lemma b_op_closed: maxvar b_op = 0.
 Proof. 
 unfold b_op. 
 rewrite maxvar_app_comb. 
-rewrite Y_k_closed. 2: omega. unfold max. 
+rewrite Y_k_closed. unfold max. 
 eapply2 b_fn_closed.
 Qed.
 
@@ -428,7 +494,7 @@ Qed.
 Lemma abs2_red : forall M N, sf_red (App (App abs_op M) N) 
 (app_comb2
      (app_comb
-        (app_comb (A_k 3)
+        (app_comb (A_k 1)
            (star_opt
               (star_opt
                  (star_opt (App (App (App b_op (Ref 0)) (Ref 2)) (Ref 1))))))
