Tree_calculus/offcuts.v
@@ -1,4 +1,430 @@
 
+
+
+Ltac eval1 := 
+unfold sf_red; 
+match goal with 
+| |- multi_step sf_red1  (App (App (App (App _ _) _) _) _) _ =>  
+eapply transitive_red; [eapply preserves_app_sf_red ; [eval1 |]|]
+| |- multi_step sf_red1  (App (App (App (Op Node) (Op Node)) _) _) _ => 
+  eapply succ_red; [eapply2 k_red |]
+| |- multi_step sf_red1  (App (App (App (Op Node) (App (Op Node) _)) _) _) _ => 
+  eapply succ_red; [eapply2 s_red |]
+| |- multi_step sf_red1  (App (App (App (Op Node) (App (App (Op Node) _) _)) _) _) _ => 
+  eapply succ_red; [eapply2 f_red |]
+| |- multi_step sf_red1  (App (App (Op Node) _) _) _ => eapply transitive_red; [eapply preserves_app_sf_red ; eval1 |]
+| |- multi_step sf_red1  (App (Op Node) _) _ => eapply transitive_red; [eapply preserves_app_sf_red ; [auto|eval1 ]|]
+| _ => auto
+end.
+
+Definition s_op := 
+star (star (star (App (App (Ref 2) (Ref 0)) 
+                                  (App (Ref 1) (Ref 0))))).
+
+(* s_opt rule takes 11 steps *) 
+
+Lemma s_op_rule : forall M N P, sf_red (App (App (App s_op M) N) P) (App (App M P) (App N P)).
+Proof.
+intros; unfold s_op; simpl; unfold_op; simpl.  
+eval1. eval1. eval1. auto.  eval1. eval1. auto. eval1. eval1. eval1. auto.  eval1. eval1. auto.  eval1. eval1. eval1. 
+ auto. eval1. eval1. auto.  eval1. eval1. eval1. auto. eval1. auto. auto.  eval1. eval1. auto.  eval1.
+auto.  auto. auto. auto. 
+ eval1. eval1. eval1. auto. 
+eval1. eval1. auto.  eval1. eval1. eval1. auto. eval1. auto. auto.  eval1. auto. auto. auto. auto. 
+  eval1. eval1. eval1. auto. eval1. auto. auto. eval1. auto. auto. auto. auto. auto. auto.   
+eval1. eval1. auto.  eval1. eval1. eval1. auto. eval1. auto. auto.  eval1. auto. auto. 
+ eval1. auto.  eval1. eval1. auto.  eval1.  eval1. eval1. auto.  eval1. eval1. auto. eval1. eval1. eval1. auto. eval1. 
+eval1. auto. eval1. eval1. eval1. auto. eval1. eval1. auto. eval1. eval1. eval1. auto.  eval1. 
+auto. auto. eval1. auto. auto. auto. auto.  eval1. eval1. eval1. auto. eval1. auto. auto.  eval1. auto. 
+auto. auto. auto. auto.  eval1.  eval1. eval1. auto.  eval1. eval1. auto.  eval1. eval1.  eval1.  auto.   
+eval1. eval1. auto.  eval1. eval1.  eval1. auto. eval1. auto. auto.  eval1. auto. auto. auto. auto. 
+ eval1. eval1. eval1. auto.  eval1. all: auto. 
+ eval1. eval1. eval1.  eval1. auto. eval1. eval1. auto. eval1. eval1. eval1. auto.
+(* 100 steps *) 
+ eval1. eval1. auto.  eval1. eval1. eval1. auto.  eval1.
+eval1. auto. eval1. eval1. eval1. auto.  eval1. eval1. auto. eval1. eval1. eval1. auto. eval1. eval1. auto.
+eval1. all: auto.
+ eval1. eval1. eval1. eval1. auto. eval1. all:auto.
+ eval1. eval1. auto. eval1. eval1.
+eval1. eval1. auto. eval1. all: auto. 
+(* 1 *) 
+eapply transitive_red; [eapply preserves_app_sf_red ; [eval1 |]|].
+eval1. auto.  eval1. eval1.  eval1. eval1. auto. eval1. eval1. auto. 
+eval1. eval1. eval1. auto. eval1. eval1. auto. eval1. eval1. eval1. auto. 
+eval1. eval1. all: auto. 
+ eval1. eval1. eval1. auto. eval1. eval1. eval1. eval1. all: auto. 
+eval1. eval1. eval1. eval1. eval1. auto. eval1. all: auto. 
+eval1. eval1. eval1. auto. eval1. eval1. eval1. eval1. all: auto.
+(* 68 steps *) 
+(* 1 *) 
+eapply transitive_red. 
+eapply preserves_app_sf_red. 
+eapply preserves_app_sf_red. 
+eapply preserves_app_sf_red. 
+eapply preserves_app_sf_red. auto. 
+eval1. eval1. eval1. eval1. eval1. eval1. auto.  eval1. auto. auto. eval1. auto. auto. auto.   
+eval1. auto.  eval1. eval1. eval1. auto.  eval1. auto. auto.  auto. eval1. eval1. auto. 
+eval1. auto. auto. auto. eval1. auto. eval1. auto. eval1. auto. eval1. auto. eval1. auto. eval1.
+auto.  eval1. auto. 
+eapply transitive_red. 
+eapply preserves_app_sf_red. 
+eapply preserves_app_sf_red. 
+eapply preserves_app_sf_red. 
+eapply preserves_app_sf_red. auto. 
+eval1. auto.  eval1. auto. auto. auto.  eval1. auto. auto. auto.  eval1. eval1. eval1. auto.
+  eval1. auto. auto. eval1. auto. auto. auto.
+eapply transitive_red. 
+eapply preserves_app_sf_red. 
+eapply preserves_app_sf_red. 
+eapply preserves_app_sf_red. auto. 
+eval1. eval1. eval1. eval1. eval1. auto. eval1. eval1. auto. eval1. eval1. eval1. auto. 
+eval1. eval1. auto.  eval1. eval1.  eval1.  auto. eval1.  auto.  auto. eval1. auto. auto. auto. 
+auto.  eval1. eval1. eval1. auto. eval1. auto. auto. eval1. all: auto. 
+eval1. eval1. auto. eval1. eval1. auto. auto. eval1.
+eapply2 preserves_app_sf_red. 
+eapply transitive_red. 
+eapply preserves_app_sf_red. 
+eapply preserves_app_sf_red. 
+eapply preserves_app_sf_red. auto. 
+eval1. eval1. eval1. eval1. eval1. auto. eval1. auto. auto.  eval1. auto. auto. auto.  eval1. auto. eval1.
+ eval1. auto. eval1. auto. auto. auto.  eval1. eval1. eval1. auto.  eval1. eval1.  auto. eval1.
+eval1. eval1. auto. eval1. auto. auto. eval1. auto. auto. auto. auto.
+eval1. eval1. eval1. auto. eval1. auto. auto. eval1. auto. auto. auto. auto. 
+eval1. eval1.  auto. eval1. auto. auto. auto.
+eapply transitive_red. 
+eapply preserves_app_sf_red. 
+eapply preserves_app_sf_red. 
+eapply preserves_app_sf_red.
+eapply preserves_app_sf_red. auto. 
+eval1. auto.  eval1. auto. auto. auto. eval1. auto. auto. auto. eval1. eval1. eval1.
+eval1. auto. eval1. eval1. auto. eval1. eval1. eval1. auto. eval1. all: auto. 
+(* 100 steps *) 
+eval1. eval1. eval1. eval1. eval1. auto. eval1. auto. auto. eval1. auto. auto. auto.  
+eval1. auto. eval1. eval1. auto. auto. eval1. eval1.
+eval1. auto.  eval1. all: auto. 
+eval1. eval1. auto.  eval1. eval1. auto. auto.
+(* 18 steps *) 
+Qed. 
+
+
+
+Definition s_opt := 
+star_opt (star_opt (star_opt (App (App (Ref 2) (Ref 0)) 
+                                  (App (Ref 1) (Ref 0))))).
+
+(* s_opt rule takes 11 steps *) 
+
+Lemma s_opt_rule : forall M N P, sf_red (App (App (App s_opt M) N) P) (App (App M P) (App N P)).
+Proof.
+intros; unfold s_opt. simpl. unfold_op; unfold subst; simpl.
+eapply succ_red. eapply app_sf_red.  eapply app_sf_red.  eapply2 s_red. auto. auto.  
+eapply succ_red. eapply app_sf_red. eapply app_sf_red.  eapply app_sf_red.  eapply2 s_red.
+eapply2 k_red.  auto.  auto. auto.
+eapply succ_red. eapply app_sf_red. eapply app_sf_red. eapply app_sf_red.  eapply app_sf_red.  eapply2 k_red.
+eapply2 s_red.  auto. auto. auto. 
+eapply succ_red. eapply app_sf_red.  eapply app_sf_red.  eapply app_sf_red.  eapply app_sf_red.   auto.  eapply app_sf_red.  eapply2 k_red. auto. auto. auto. auto.
+eapply succ_red. eapply app_sf_red.  eapply2 s_red. auto. 
+eapply succ_red. eapply app_sf_red.  eapply app_sf_red.  eapply s_red. auto. auto. auto. 
+eapply2 k_red. auto.
+eapply succ_red.   eapply app_sf_red.  eapply app_sf_red. eapply app_sf_red.   eapply2 k_red. auto. auto. auto.
+eapply succ_red.  eapply s_red. all: auto. 
+Qed. 
+
+  
+
+
+Lemma maxvar_occurs: forall M, maxvar M = 1 -> occurs 0 M >0. 
+Proof.
+induction M; split_all.
+gen_case H n.  omega.
+assert(maxvar M1 = 1 \/ maxvar M2 = 1). 
+gen_case H (maxvar M1).
+gen_case H (maxvar M2).
+assert (max n n0 >= n) by eapply2 max_is_max.
+left; omega. 
+inversion H0. 
+assert(occurs 0 M1 >0) by eapply2 IHM1. omega. 
+assert(occurs 0 M2 >0) by eapply2 IHM2. omega. 
+Qed.  
+
+
+(*
+(* A4 *) 
+
+
+Definition A41 M := (star_opt (app_comb (A_k 3) (app_comb (lift 1 M) (Ref 0)))).
+
+
+Lemma A4_red1: forall M, sf_red (App (A_k 4) M) (A41 M).
+Proof.
+intros. 
+replace (A_k 4) with (star_opt (star_opt (app_comb (A_k 3) (app_comb (Ref 1) (Ref 0)))))
+by (unfold A_k; auto).
+eapply transitive_red. 
+eapply2 star_opt_beta. 
+unfold subst. 
+rewrite subst_rec_preserves_star_opt.
+rewrite ! subst_rec_preserves_app_comb.
+rewrite subst_rec_closed. 
+2: rewrite A_k_closed; split_all.
+unfold subst_rec.  insert_Ref_out. 
+eapply2 zero_red. 
+Qed. 
+
+
+Definition A42 M N := app_comb (A_k 3) (app_comb M N).
+ 
+Lemma A4_red2: forall M N, sf_red (App (A41 M) N) (A42 M N).
+Proof.
+intros; unfold A41.  
+eapply transitive_red. 
+eapply2 star_opt_beta.
+unfold subst; rewrite ! subst_rec_preserves_app_comb.
+unfold lift; 
+rewrite subst_rec_lift_rec; try omega.
+rewrite subst_rec_ref. 
+rewrite subst_rec_closed. 
+2: rewrite A_k_closed; auto. 
+insert_Ref_out. 
+unfold lift; rewrite ! lift_rec_null.
+eapply2 zero_red.
+Qed. 
+
+ 
+Definition A43 M N P :=  A32 (app_comb M N) P. 
+
+Lemma A4_red3: forall M N P, sf_red (App (A42 M N) P) (A43 M N P).
+Proof.
+intros; unfold A42.
+eapply transitive_red.
+eapply2 app_comb_red. 
+eapply transitive_red. 
+eapply preserves_app_sf_red.
+eapply2 A3_red1. auto. 
+eapply2 A3_red2.   
+Qed. 
+
+  
+Definition A44 M N P Q := A33 (app_comb M N) P Q.
+
+Lemma A4_red4 : forall M N P Q, 
+sf_red (App (A43 M N P) Q) (A44 M N P Q). 
+Proof. 
+intros. unfold A43. 
+eapply2 A3_red3. 
+Qed. 
+
+Lemma A4_red5 : forall M N P Q R, 
+sf_red (App (A44 M N P Q) R) (App (App (App (App M N) P) Q) R).
+Proof. 
+intros. unfold A44.
+eapply transitive_red.
+eapply2 A3_red4.  
+eapply transitive_red. eapply preserves_app_sf_red. eapply preserves_app_sf_red. 
+eapply2 app_comb_red. auto. auto. auto. 
+Qed. 
+
+Lemma A5_red: forall M N P Q R, 
+sf_red (App (App (App (App (App (A_k 5) M) N) P) Q) R) (App (App (App (App M N) P) Q) R) .
+Proof. 
+intros. 
+eapply transitive_red. 
+eapply preserves_app_sf_red. 
+eapply preserves_app_sf_red. 
+eapply preserves_app_sf_red. 
+instantiate(1:= app_comb (A_k 4) (app_comb M N)).
+unfold A_k; auto.
+eapply transitive_red.  
+eapply star_opt_beta2. 
+unfold subst; 
+rewrite ! subst_rec_preserves_app_comb.
+rewrite ! subst_rec_preserves_star_opt.
+rewrite ! subst_rec_preserves_app_comb.
+rewrite ! subst_rec_preserves_star_opt.
+rewrite ! subst_rec_preserves_app_comb.
+unfold subst_rec; fold subst_rec. 
+insert_Ref_out. 
+unfold subst_rec; fold subst_rec. 
+insert_Ref_out. 
+unfold lift; rewrite ! lift_rec_null. 
+rewrite subst_rec_lift_rec; try omega. 
+rewrite ! subst_rec_closed. 
+2: unfold_op; simpl; auto. 
+2: unfold_op; simpl; auto. 
+all: auto. 
+rewrite lift_rec_null. auto. 
+(* 1 *) 
+eapply transitive_red. 
+eapply preserves_app_sf_red. 
+eapply preserves_app_sf_red. 
+eapply2 app_comb_red. 
+all: auto. 
+eapply transitive_red. 
+eapply preserves_app_sf_red. 
+eapply preserves_app_sf_red. 
+eapply preserves_app_sf_red. 
+eapply2 A4_red1.
+all: auto. 
+eapply transitive_red. 
+eapply preserves_app_sf_red. 
+eapply preserves_app_sf_red. 
+eapply2 A4_red2.
+all: auto. 
+eapply transitive_red. 
+eapply preserves_app_sf_red. 
+eapply2 A4_red3.  all: auto. 
+eapply transitive_red.
+ eapply2 A4_red4.
+unfold A44. unfold A33.  preserves_app_sf_red. 
+instantiate(1:= app_comb (A_k 4) (app_comb M N)).
+unfold A_k; auto.
+eapply transitive_red.  
+eapply star_opt_beta2. 
+unfold subst; 
+rewrite ! subst_rec_preserves_app_comb.
+rewrite ! subst_rec_preserves_star_opt.
+rewrite ! subst_rec_preserves_app_comb.
+rewrite ! subst_rec_preserves_star_opt.
+rewrite ! subst_rec_preserves_app_comb.
+unfold subst_rec; fold subst_rec. 
+insert_Ref_out. 
+unfold subst_rec; fold subst_rec. 
+insert_Ref_out. 
+unfold lift; rewrite ! lift_rec_null. 
+rewrite subst_rec_lift_rec; try omega. 
+rewrite ! subst_rec_closed. 
+2: unfold_op; simpl; auto. 
+2: unfold_op; simpl; auto. 
+all: auto. 
+rewrite lift_rec_null. auto. 
+
+
+
+
+unfold A_k; fold A_k. 
+
+*) 
+(* 
+Lemma aux :
+  forall M N, occurs 0 M >0 -> maxvar N = 0 -> S (size(subst M N)) >= size M + size N.
+Proof.
+  induction M; split_all.
+  gen_case H n. unfold subst; simpl. insert_Ref_out.
+  unfold lift; rewrite lift_rec_null. omega. omega. omega. 
+  assert(occurs 0 M1 >0 \/ occurs 0 M2 >0) by omega.
+  inversion H1.
+  assert(S(size (subst M1 N)) >= size M1 + size N) by eapply2 IHM1.   
+  unfold subst in *.
+assert(size (subst_rec M2 N 0) >= size M2). apply size_subst. ga.   
+*) 
+
+
+(* restore ? 
+Lemma star_bigger: 
+forall M, maxvar M = 0 -> 
+star_opt
+  (star_opt
+     (App (Ref 0)
+        (app_comb (app_comb (app_comb M (Ref 1)) (Ref 1)) (Ref 0)))) <>
+M. 
+Proof.
+  intros. 
+  replace (star_opt (star_opt (App (Ref 0) (app_comb (app_comb (app_comb M (Ref 1)) (Ref 1)) (Ref 0)))))
+  with
+    (subst (star_opt (star_opt (App (Ref 0) (app_comb (app_comb (app_comb (Ref 2) (Ref 1)) (Ref 1)) (Ref 0))))) M) .
+  intro. 
+elim(size_subst_star_opt (star_opt
+               (App (Ref 0)
+                  (app_comb (app_comb (app_comb (Ref 2) (Ref 1)) (Ref 1)) (Ref 0)))) M); intros; auto. 
+
+  unfold app_comb, star_opt; unfold_op; unfold occurs, eqnat; simpl. 
+intro.
+omega. intro.
+
+
+  
+intros. 
+rewrite star_opt_occurs_true. 
+2: cbv. 2: omega.
+2: discriminate . 
+unfold star_opt at 3.
+unfold app_comb.
+rewrite  (star_opt_occurs_true (App (Op Node) (App (Op Node) i_op))). 
+2: unfold app_comb; simpl; auto. 2: omega. 
+2: discriminate . 
+ rewrite  (star_opt_occurs_true (App (Op Node) (App (Op Node) (App k_op (Ref 0))))). 
+2: unfold app_comb; simpl; auto. 2: omega. 
+2: discriminate .
+rewrite (star_opt_occurs_false (App k_op _)). 
+2: simpl; auto. 2: eapply2 occurs_closed; auto.
+subst_tac.
+rewrite subst_rec_closed. 2: omega. 
+rewrite star_opt_occurs_true. 
+2: simpl; auto. 2: omega. 2: discriminate.
+rewrite star_opt_closed. 2: cbv; omega.
+rewrite star_opt_occurs_true.
+2: unfold app_comb; simpl; auto. 2: omega. 
+2: discriminate .
+rewrite star_opt_occurs_true.
+2: unfold app_comb; simpl; auto.
+2: discriminate .
+rewrite star_opt_occurs_true.
+2: unfold app_comb; simpl; auto.
+2: discriminate .
+rewrite star_opt_closed.
+2: cbv; auto. 
+rewrite star_opt_occurs_true.
+2: unfold app_comb; simpl; auto.
+2: discriminate .
+rewrite star_opt_occurs_true.
+2: unfold app_comb; simpl; auto.
+2: discriminate .
+rewrite star_opt_occurs_true.
+2: unfold app_comb; simpl; auto.
+2: discriminate .
+rewrite star_opt_closed.
+2: cbv; auto. 
+rewrite star_opt_occurs_true.
+2: unfold app_comb; simpl; auto.
+2: discriminate .
+rewrite star_opt_occurs_true.
+2: unfold app_comb; simpl; auto.
+2: discriminate .
+rewrite star_opt_occurs_true.
+2: unfold app_comb; simpl; auto.
+2: discriminate .
+rewrite star_opt_occurs_true.
+2: unfold app_comb; simpl; auto.
+2: discriminate .
+rewrite star_opt_occurs_true.
+2: unfold app_comb; simpl; auto.
+2: discriminate .
+rewrite star_opt_occurs_true.
+2: unfold app_comb; simpl; auto.
+2: discriminate .
+rewrite star_opt_occurs_true.
+2: unfold app_comb; simpl; auto.
+2: discriminate .
+rewrite star_opt_occurs_true.
+2: unfold app_comb; simpl; auto.
+2: discriminate .
+rewrite star_opt_occurs_true.
+2: unfold app_comb; simpl; auto.
+2: discriminate .
+rewrite star_opt_closed.
+2: cbv; auto. 
+intro. clear H.  
+match goal with 
+| H: ?M = ?N |- _ => assert(size M = size N) by congruence 
+end.
+clear H0.
+generalize H. clear H. unfold_op; unfold star_opt, occurs, size; fold size.
+rewrite ! orb_false_l. 
+unfold_op; unfold subst, subst_rec, size; fold size. 
+intro; omega.
+Qed. 
+ *)
+
 (* 
 Lemma star_opt_app_comb2:
   forall M N, maxvar M = 0 -> occurs 0 N = true -> occurs 1 N = true -> 
