Tree_calculus/Abstraction5.v
@@ -1,0 +1,1501 @@
+(**********************************************************************)
+(* This Program is free software; you can redistribute it and/or      *)
+(* modify it under the terms of the GNU Lesser General Public License *)
+(* as published by the Free Software Foundation; either version 2.1   *)
+(* of the License, or (at your option) any later version.             *)
+(*                                                                    *)
+(* This program is distributed in the hope that it will be useful,    *)
+(* but WITHOUT ANY WARRANTY; without even the implied warranty of     *)
+(* MERCHANTABILITY or FITNESS FOR A PARTICULAR PURPOSE.  See the      *)
+(* GNU General Public License for more details.                       *)
+(*                                                                    *)
+(* You should have received a copy of the GNU Lesser General Public   *)
+(* License along with this program; if not, write to the Free         *)
+(* Software Foundation, Inc., 51 Franklin St, Fifth Floor, Boston, MA *)
+(* 021101301 USA                                                     *)
+(**********************************************************************)
+
+(**********************************************************************)
+(*                 Abstraction_to_Tree.v                              *)
+(*                                                                    *)
+(*                     Barry Jay                                      *)
+(*                                                                    *)
+(**********************************************************************)
+
+
+Require Import Omega Max Bool List.
+Require Import IntensionalLib.SF_calculus.Test.  
+Require Import IntensionalLib.SF_calculus.General.  
+Require Import IntensionalLib.Tree_calculus.Abstraction_Terms.  
+Require Import IntensionalLib.Tree_calculus.Abstraction_Reduction.  
+Require Import IntensionalLib.Tree_calculus.Tree_Terms.  
+Require Import IntensionalLib.Tree_calculus.Tree_Tactics.  
+Require Import IntensionalLib.Tree_calculus.Tree_reduction.  
+Require Import IntensionalLib.Tree_calculus.Tree_Normal.  
+Require Import IntensionalLib.Tree_calculus.Tree_Closed.  
+Require Import IntensionalLib.Tree_calculus.Substitution.  
+Require Import IntensionalLib.Tree_calculus.Tree_Eval.  
+Require Import IntensionalLib.Tree_calculus.Star.  
+Require Import IntensionalLib.Tree_calculus.Wait.  
+Require Import IntensionalLib.Tree_calculus.Fixpoints.  
+Require Import IntensionalLib.Tree_calculus.Wave_Factor.  
+Require Import IntensionalLib.Tree_calculus.Wave_Factor2.  
+Require Import IntensionalLib.Tree_calculus.Equal.  
+Require Import IntensionalLib.Tree_calculus.Case.  
+Require Import IntensionalLib.Tree_calculus.Extensions.  
+Require Import IntensionalLib.Tree_calculus.Wait2.  
+Require Import IntensionalLib.Tree_calculus.Abstraction.  
+Require Import IntensionalLib.Tree_calculus.Abstraction2.  
+Require Import IntensionalLib.Tree_calculus.Abstraction3. 
+Require Import IntensionalLib.Tree_calculus.occurs. 
+
+
+
+Lemma b_h_op_red: forall M N, sf_red (App (App (App b_op M) N) h_op) h_op.
+Proof.
+intros; unfold b_op. 
+eapply transitive_red. 
+eapply preserves_app_sf_red.
+eapply preserves_app_sf_red.
+eapply2 app_comb_red. all: auto. 
+eapply transitive_red.    
+eapply2 Y2_fix.
+unfold b_fn at 1. 
+eapply transitive_red.
+eapply preserves_app_sf_red. 
+eapply2 star_opt_beta3. auto. 
+unfold subst.
+rewrite ! subst_rec_preserves_extension.
+(* 1 *) 
+eapply transitive_red. 
+eapply2 extensions_by_matchfail.
+eapply2 matchfail_app_comb_l.
+eapply2 matchfail_app_comb_l.
+eapply2 matchfail_app_comb_r.
+eapply2 matchfail_program. 
+eapply2 h_fn_program.
+split. eapply2 omega_k_normal. eapply2 omega_k_closed.
+eapply2 h_fn_not_omega. 
+(* 1 *) 
+eapply transitive_red. 
+eapply2 extensions_by_matchfail.
+eapply2 matchfail_app_comb_l.
+eapply2 matchfail_app_comb_l.
+eapply2 matchfail_app_comb_l.
+eapply2 matchfail_program.
+split. apply app_comb_normal. eapply2 omega_k_normal. eapply2 omega_k_normal.
+rewrite maxvar_app_comb. rewrite ! omega_k_closed. auto.
+split. eapply2 A_k_normal. eapply2 A_k_closed.
+discriminate. 
+(* 1 *) 
+eapply transitive_red. 
+eapply2 extensions_by_matchfail.
+eapply2 matchfail_app_comb_l.
+eapply2 matchfail_app_comb_l.
+eapply2 matchfail_app_comb_r.
+eapply2 matchfail_program.
+split. eapply2 omega_k_normal. eapply2 omega_k_closed.
+split. eapply2 omega_k_normal. eapply2 omega_k_closed.
+replace 4 with (S (3 +0)) by auto. 
+replace 2 with (S (0+1)) by omega.
+eapply2 omega_k_mono. 
+(* 1 *) 
+eapply transitive_red. 
+eapply2 extensions_by_matchfail.
+eapply2 matchfail_app_comb_l.
+eapply2 matchfail_app_comb_r.
+eapply2 matchfail_program. 
+split. eapply2 omega_k_normal. eapply2 omega_k_closed.
+split. eapply2 omega_k_normal. eapply2 omega_k_closed.
+replace 2 with (S(1+0)) by auto.
+eapply2 omega_k_mono.  
+(* 1 *) 
+eapply transitive_red. 
+eapply2 extensions_by_matchfail.
+eapply2 matchfail_app_comb_r.
+unfold h_fn.
+rewrite star_opt_eta. 
+2: simpl; auto.
+unfold subst, subst_rec. insert_Ref_out. unfold pred.   
+rewrite star_opt_occurs_true. 
+2: simpl; auto. 2: discriminate. 
+rewrite star_opt_eta.  2: auto. 
+rewrite star_opt_occurs_true. 
+2: simpl; auto. 2: discriminate.
+unfold subst, subst_rec; insert_Ref_out. unfold pred.
+rewrite star_opt_occurs_true. 
+2: simpl; auto. 2: discriminate. 
+eapply2 matchfail_compound_l.
+eapply2 matchfail_compound_r.
+eapply2 matchfail_compound_r.
+apply matchfail_program. 
+unfold_op; split; auto.
+cbv; split; auto.
+repeat eapply2 nf_compound.
+discriminate.
+(* 1 *) 
+eapply transitive_red. 
+eapply2 extensions_by_matchfail. 
+unfold h_op, ab1. 
+eapply2 matchfail_compound_l.
+eapply2 matchfail_compound_r.
+eapply2 matchfail_compound_r.
+eapply2 matchfail_compound_l.
+unfold_op. 
+eapply2 matchfail_compound_r.
+(* 1 *) 
+eapply transitive_red. 
+eapply2 extensions_by_matchfail. 
+unfold h_op. 
+eapply2 matchfail_app_comb_r.
+unfold h_fn. 
+rewrite star_opt_eta. 2: cbv; auto. repeat subst_tac.
+eapply2 matchfail_compound_l. simpl. unfold_op. subst_tac. 
+eapply2 matchfail_compound_r.
+eapply2 matchfail_compound_r.
+eapply2 matchfail_compound_l.
+eapply2 matchfail_compound_r. 
+eapply2 matchfail_compound_r. 
+eapply2 matchfail_op. 
+right; auto. 
+discriminate . 
+(* 1 *) 
+unfold_op; simpl. eval_tac. eval_tac.   
+Qed. 
+
+
+
+Lemma app_comb_vs_abs_op: forall M N, 
+matchfail
+  (app_comb M N) abs_op.
+Proof. 
+intros.
+unfold abs_op, ab_op, app_comb2.
+unfold app_comb at 2.
+rewrite star_opt_occurs_true. 
+all: cycle 1. 
+unfold flip, app_comb; unfold_op. 
+rewrite ! occurs_app.
+replace (occurs 0 (Ref 0)) with 1 by auto. omega. 
+discriminate. 
+(* 1 *) 
+rewrite star_opt_occurs_true.
+eapply2 matchfail_compound_l. 
+eapply2 matchfail_compound_r. 
+eapply2 matchfail_compound_r. 
+eapply2 matchfail_compound_l. 
+unfold_op; auto. eapply2 matchfail_compound_r. 
+unfold_op; auto. 
+unfold_op; auto. 
+unfold flip; rewrite ! occurs_app. 
+assert(occurs 0
+     (star_opt
+        (App
+           (App (Op Node)
+              (App (Op Node)
+                 (App k_op (app_comb (app_comb (A_k 1) (ab_fn b_op)) (Ref 1)))))
+           (App k_op (App (App node (App node (App k_op (Ref 0)))) i_op)))) =1).
+all: cycle 1. rewrite H; omega. 
+discriminate.
+(* 1 *) 
+rewrite (star_opt_occurs_true) at 1.
+all: cycle 1. 
+rewrite ! occurs_app.
+replace (occurs 0 (Ref 0)) with 1 by auto. omega. 
+discriminate.
+rewrite ! occurs_app. 
+assert(occurs 0
+    (star_opt
+       (App (Op Node)
+            (App (Op Node) (App k_op (app_comb (app_comb (A_k 1) (ab_fn b_op)) (Ref 1)))))) = 1).
+2: rewrite H; cbv; omega. 
+rewrite (star_opt_occurs_false).
+all: cycle 1. 
+unfold app_comb; unfold_op. rewrite ! occurs_app.
+rewrite (occurs_closed 0 (A_k 1)). 
+2: apply A_k_closed.
+rewrite (occurs_closed 0 (ab_fn b_op)).
+cbv; auto. apply ab_fn_program. apply b_op_program.
+subst_tac. rewrite ! subst_rec_preserves_app_comb.
+rewrite subst_rec_closed. 2: rewrite A_k_closed; omega.
+rewrite subst_rec_closed.
+rewrite occurs_app. subst_tac. 
+unfold app_comb. rewrite ! occurs_app. 
+replace (occurs 0 (Ref 0)) with 1 by auto.
+rewrite (occurs_closed 0 (ab_fn b_op)).
+cbv; auto. apply ab_fn_program. apply b_op_program.
+cut(maxvar (ab_fn b_op) = 0). intros; omega. 
+apply ab_fn_program. apply b_op_program.
+Qed.
+
+Lemma b_abs_op_red: forall M N, sf_red (App (App (App b_op M) N) abs_op) abs_op.
+Proof.
+intros; unfold b_op. 
+eapply transitive_red. 
+eapply preserves_app_sf_red.
+eapply preserves_app_sf_red.
+eapply2 app_comb_red. auto. auto.  
+eapply transitive_red.    
+eapply2 Y2_fix.
+unfold b_fn at 1. 
+eapply transitive_red.
+eapply preserves_app_sf_red. 
+eapply2 star_opt_beta3. auto. 
+unfold subst.
+rewrite ! subst_rec_preserves_extension.
+(* 1 *) 
+eapply transitive_red. 
+eapply2 extensions_by_matchfail.
+eapply2 app_comb_vs_abs_op. 
+(* 1 *) 
+eapply transitive_red. 
+apply extensions_by_matchfail.  
+eapply2 app_comb_vs_abs_op.
+(* 1 *)  
+eapply transitive_red. 
+apply extensions_by_matchfail.  
+eapply2 app_comb_vs_abs_op.
+(* 1 *)  
+eapply transitive_red. 
+apply extensions_by_matchfail.  
+eapply2 app_comb_vs_abs_op.
+eapply transitive_red. 
+apply extensions_by_matchfail.  
+eapply2 app_comb_vs_abs_op.
+(* 1 *) 
+eapply transitive_red. 
+eapply2 extensions_by_matchfail. 
+unfold abs_op, ab_op. 
+unfold app_comb2, flip.
+unfold app_comb at 1. 
+(* 2 *) 
+rewrite star_opt_occurs_true.
+all: cycle 1. 
+unfold_op. 
+rewrite ! occurs_app.
+replace (occurs 0 (Ref 0)) with 1 by auto. omega. 
+discriminate. 
+(* 2 *) 
+eapply transitive_red. 
+eapply2 extensions_by_matchfail. 
+unfold abs_op, ab_op. 
+unfold app_comb2, flip.
+unfold app_comb at 5. 
+(* 3 *) 
+rewrite star_opt_occurs_true.
+all: cycle 1. 
+unfold_op. 
+rewrite ! occurs_app.
+replace (occurs 0 (Ref 0)) with 1 by auto; omega. 
+discriminate. 
+(* 1 *) 
+all: cycle -1. 
+rewrite star_opt_occurs_true. 
+all: cycle 1. 
+unfold_op. 
+rewrite ! occurs_app.
+rewrite occurs_star_opt.
+rewrite ! occurs_app. 
+replace (occurs 1 (Ref 1)) with 1 by auto. omega. 
+discriminate.
+(* 1 *) 
+all: cycle -1. 
+eapply2 matchfail_compound_l. 
+eapply2 matchfail_compound_r. 
+eapply2 matchfail_compound_r. 
+eapply2 matchfail_compound_l.
+unfold_op; auto.
+unfold_op; auto.   
+eapply2 matchfail_compound_r.
+(* 2 *) 
+all: cycle -1. 
+rewrite (star_opt_occurs_true (App (Op Node)
+                       (App (Op Node)
+                          (App k_op
+                             (app_comb (app_comb (A_k 1) (ab_fn b_op))
+                                (Ref 1)))))) at 1.
+all: cycle 1. 
+unfold_op. 
+rewrite ! occurs_app.
+replace (occurs 0 (Ref 0)) with 1 by auto. omega. 
+discriminate. 
+(* 2 *) 
+all: cycle -1.
+unfold_op.
+rewrite star_opt_occurs_true. 
+all: cycle 1. 
+unfold_op. 
+rewrite ! occurs_app.
+rewrite ! occurs_star_opt. 
+rewrite ! occurs_app.
+replace (occurs 1 (Ref 1)) with 1  by auto. omega. 
+discriminate. 
+all: cycle -1 . 
+(* 2 *)  
+eapply2 matchfail_compound_l. 
+eapply2 matchfail_compound_r. 
+eapply2 matchfail_compound_r. 
+eapply2 matchfail_compound_l.
+unfold_op; auto.
+eapply2 matchfail_compound_r.
+unfold_op; auto. 
+unfold_op. 
+eapply2 matchfail_compound_op.
+(* 1 *)  
+unfold_op; simpl. 
+eapply succ_red. eapply2 s_red. 
+eapply succ_red. eapply k_red.
+auto. 
+auto.
+Qed. 
+
+Lemma b_i_op_red: forall M N, sf_red (App (App (App b_op M) N) i_op) i_op.
+Proof.
+intros; unfold b_op. 
+eapply transitive_red. 
+eapply preserves_app_sf_red.
+eapply preserves_app_sf_red.
+eapply2 app_comb_red. all: auto. 
+eapply transitive_red.    
+eapply2 Y2_fix.
+unfold b_fn at 1. 
+eapply transitive_red.
+eapply preserves_app_sf_red. 
+eapply2 star_opt_beta3. auto. 
+unfold subst.
+rewrite ! subst_rec_preserves_extension.
+(* 1 *) 
+eapply transitive_red. 
+eapply2 extensions_by_matchfail.
+eapply2 app_comb_vs_I. 
+(* 1 *) 
+eapply transitive_red. 
+eapply2 extensions_by_matchfail.
+eapply2 app_comb_vs_I. 
+(* 1 *) 
+eapply transitive_red. 
+eapply2 extensions_by_matchfail.
+eapply2 app_comb_vs_I. 
+(* 1 *) 
+eapply transitive_red. 
+eapply2 extensions_by_matchfail.
+eapply2 app_comb_vs_I. 
+(* 1 *) 
+eapply transitive_red. 
+eapply2 extensions_by_matchfail.
+eapply2 app_comb_vs_I. 
+(* 1 *) 
+eapply transitive_red. 
+eapply2 extensions_by_matchfail.
+unfold ab1.  unfold_op. 
+eapply2 matchfail_compound_l. 
+(* 1 *) 
+eapply transitive_red. 
+eapply2 extensions_by_matchfail.
+unfold_op; eapply2 matchfail_compound_l. 
+(* 1 *) 
+unfold_op; simpl. repeat eval_tac. 
+Qed. 
+
+Lemma occur_ref: forall n k, occurs k (Ref n) = eqnat n k. 
+Proof. auto. Qed.  
+
+Lemma b_b_op_red: forall M N, sf_red (App (App (App b_op M) N) b_op) b_op.
+Proof.
+intros; unfold b_op. 
+eapply transitive_red. 
+eapply preserves_app_sf_red.
+eapply preserves_app_sf_red.
+eapply2 app_comb_red. all: auto. 
+eapply transitive_red.    
+eapply2 Y2_fix.
+unfold b_fn at 1. 
+eapply transitive_red.
+eapply preserves_app_sf_red. 
+eapply2 star_opt_beta3. auto. 
+unfold subst.
+rewrite ! subst_rec_preserves_extension.
+(* 1 *) 
+eapply transitive_red. 
+eapply2 extensions_by_matchfail.
+eapply2 matchfail_app_comb_l.
+eapply2 matchfail_app_comb_l.
+eapply2 matchfail_app_comb_r.
+apply matchfail_program.
+eapply2 h_fn_program. 
+split. eapply2 omega_k_normal. eapply2 omega_k_closed. 
+eapply2 h_fn_not_omega. 
+(* 1 *) 
+eapply transitive_red. 
+eapply2 extensions_by_matchfail.
+eapply2 matchfail_app_comb_l.
+eapply2 matchfail_app_comb_l.
+eapply2 matchfail_app_comb_l.
+eapply matchfail_program. 
+eapply2 app_comb_program. 
+split. eapply2 omega_k_normal. eapply2 omega_k_closed. 
+split. eapply2 omega_k_normal. eapply2 omega_k_closed. 
+split. eapply2 A_k_normal. eapply2 A_k_closed.
+discriminate.   
+(* 1 *) 
+eapply transitive_red. 
+eapply2 extensions_by_matchfail.
+eapply2 matchfail_app_comb_l.
+eapply2 matchfail_app_comb_l.
+eapply2 matchfail_app_comb_r.
+eapply matchfail_program. 
+split. eapply2 omega_k_normal. eapply2 omega_k_closed. 
+split. eapply2 omega_k_normal. eapply2 omega_k_closed. 
+replace 2 with (S (0+1)) by auto. 
+apply omega_k_mono.
+(* 1 *) 
+eapply transitive_red. 
+eapply2 extensions_by_matchfail.
+eapply2 matchfail_app_comb_l.
+eapply2 matchfail_app_comb_r.
+eapply matchfail_program. 
+split. eapply2 omega_k_normal. eapply2 omega_k_closed. 
+split. eapply2 omega_k_normal. eapply2 omega_k_closed. 
+replace 2 with (S (1+0)) by auto. 
+apply omega_k_mono.
+(* 1 *) 
+eapply transitive_red. 
+eapply2 extensions_by_matchfail.
+eapply2 matchfail_app_comb_r.
+(* 2 *) 
+unfold b_fn.
+unfold extension at 1. 
+rewrite star_opt_occurs_true.
+all: cycle 1.
+unfold_op. 
+rewrite ! occurs_app.
+rewrite ! occurs_extension.  
+rewrite ! occurs_app.
+rewrite ! occurs_op.
+rewrite pattern_size_ab1. 
+rewrite pattern_size_app_comb2.
+rewrite ! pattern_size_app. 
+rewrite ! pattern_size_op. 
+rewrite ! pattern_size_ref.
+rewrite ! pattern_size_closed.
+all: cycle 1. 
+rewrite omega_k_closed. auto. 
+rewrite Y_k_closed. omega.  
+rewrite A_k_closed. omega.
+cbv; auto. 
+eapply2 omega_k_closed.
+discriminate. 
+all: cycle -1.
+unfold plus.
+rewrite ! occur_ref; unfold eqnat.
+omega.
+(* 2 *)
+eapply transitive_red. 
+eapply2 extensions_by_matchfail.
+(* 3 *) 
+unfold ab1. unfold_op. 
+eapply2 matchfail_compound_l. 
+eapply2 matchfail_compound_r.
+eapply2 matchfail_compound_r.
+(* 2 *) 
+eapply transitive_red. 
+eapply2 extensions_by_matchfail.
+eapply2 matchfail_app_comb_r.
+unfold b_fn.
+(* 3 *) 
+unfold extension at 1. 
+rewrite star_opt_occurs_true. 
+rewrite star_opt_occurs_true. 
+rewrite star_opt_occurs_true.
+eapply2 matchfail_compound_l. 
+eapply2 matchfail_compound_r. 
+eapply2 matchfail_compound_r.
+rewrite star_opt_occurs_true. 
+rewrite star_opt_occurs_true.
+eapply2 matchfail_compound_l. 
+eapply2 matchfail_compound_r. 
+unfold_op; auto. 
+eapply2 matchfail_compound_r.
+unfold_op; auto. 
+eapply2 matchfail_op.
+right; auto. simpl; auto. 
+unfold_op; auto. 
+discriminate. 
+(* 12 *) 
+rewrite ! occurs_app. 
+rewrite occurs_star_opt.
+rewrite ! occurs_app. 
+rewrite occurs_star_opt. 
+rewrite occurs_case. 
+rewrite ! pattern_size_app_comb.
+rewrite ! pattern_size_ref.
+rewrite ! pattern_size_closed. 
+cbv; auto. 
+eapply2 omega_k_closed.
+cbv; auto. 
+discriminate. 
+(* 10 *) 
+rewrite ! occurs_app. 
+rewrite occurs_star_opt.
+rewrite occurs_case. 
+rewrite ! pattern_size_app_comb.
+rewrite ! pattern_size_ref.
+rewrite ! pattern_size_closed. 
+cbv; auto. 
+eapply2 omega_k_closed.
+cbv; auto. 
+discriminate.
+(* 8 *) 
+rewrite ! occurs_app. 
+rewrite ! occurs_star_opt.
+rewrite ! occurs_app.
+rewrite ! occurs_extension.  
+rewrite occurs_star_opt. 
+rewrite pattern_size_ab1. 
+rewrite pattern_size_app_comb2. 
+rewrite ! pattern_size_app_comb.
+rewrite ! pattern_size_ref.
+rewrite ! pattern_size_closed.
+unfold app_comb; unfold_op. 
+rewrite ! occurs_app.
+rewrite ! occurs_op.
+rewrite ! occur_ref.
+unfold plus, eqnat.
+omega. 
+eapply2 omega_k_closed. 
+eapply2 Y_k_closed. 
+eapply2 A_k_closed. 
+cbv; auto.
+eapply2 omega_k_closed. 
+(* 7 *) 
+rewrite star_opt_occurs_true. 
+discriminate. 
+rewrite ! occurs_app.
+rewrite occurs_star_opt. 
+rewrite occurs_case. 
+rewrite ! pattern_size_app_comb. 
+rewrite ! pattern_size_ref.
+rewrite ! pattern_size_closed.
+cbv. auto. 
+eapply2 omega_k_closed.
+cbv; auto. 
+discriminate.
+(* 6 *) 
+rewrite ! occurs_app. 
+rewrite occurs_star_opt. 
+rewrite occurs_case.
+rewrite ! pattern_size_app_comb. 
+rewrite ! pattern_size_ref.
+rewrite ! pattern_size_closed.
+rewrite ! occurs_app.
+unfold occurs at 4. unfold eqnat, plus; fold plus.  omega. 
+eapply2 omega_k_closed.
+cbv; auto.
+(* 5 *) 
+rewrite star_opt_occurs_true. 
+discriminate. 
+rewrite ! occurs_app.
+rewrite ! occurs_extension.
+rewrite ! pattern_size_ab1. 
+rewrite ! pattern_size_app_comb2.  
+rewrite ! pattern_size_app_comb. 
+rewrite ! pattern_size_ref.
+rewrite ! pattern_size_closed.
+rewrite ! occurs_app.
+unfold plus; fold plus.
+replace (occurs 2 (Ref 2)) with 1 by auto.
+unfold_op; unfold occurs; fold occurs. 
+unfold eqnat, plus; fold plus. omega.
+eapply2 omega_k_closed. 
+eapply2 Y_k_closed.
+eapply2 A_k_closed. 
+cbv; auto. 
+eapply2 omega_k_closed. 
+discriminate . 
+(* 4 *) 
+rewrite ! occurs_app.
+rewrite ! occurs_extension.
+rewrite ! pattern_size_ab1. 
+rewrite ! pattern_size_app_comb2.  
+rewrite ! pattern_size_app_comb. 
+rewrite ! pattern_size_ref.
+rewrite ! pattern_size_closed.
+unfold plus; fold plus. 
+rewrite ! occurs_app.
+replace (occurs 2 (Ref 2)) with 1 by auto.
+rewrite ! occur_ref.
+unfold eqnat. 
+unfold plus; fold plus.
+omega.
+eapply2 omega_k_closed. 
+eapply2 Y_k_closed.
+eapply2 A_k_closed. 
+cbv; auto. 
+eapply2 omega_k_closed. 
+discriminate . 
+(* 2 *)
+subst_tac. eval_tac. eval_tac. 
+(* 1 *) 
+rewrite star_opt_occurs_true. 
+rewrite star_opt_occurs_true. 
+eapply2 matchfail_compound_l. 
+eapply2 matchfail_compound_r. 
+eapply2 matchfail_compound_r.
+unfold_op. 
+rewrite star_opt_occurs_true. 
+rewrite star_opt_occurs_true. 
+eapply2 matchfail_compound_l. 
+eapply2 matchfail_compound_r. 
+eapply2 matchfail_compound_r.
+eapply2 matchfail_op. 
+right; cbv; auto. 
+cbv; discriminate. 
+(* 9 *) 
+rewrite ! occurs_app.
+rewrite ! occurs_star_opt.
+rewrite ! occurs_app. 
+rewrite ! occurs_star_opt. 
+rewrite ! occurs_case. 
+rewrite ! pattern_size_app. 
+rewrite ! pattern_size_ref.
+rewrite ! pattern_size_op. 
+rewrite ! pattern_size_closed.
+cbv. auto. 
+eapply2 omega_k_closed.
+cbv; auto.
+cbv; discriminate . 
+(* 7 *)   
+rewrite ! occurs_app.
+rewrite ! occurs_star_opt.
+rewrite ! occurs_case. 
+rewrite ! pattern_size_app. 
+rewrite ! pattern_size_ref.
+rewrite ! pattern_size_op. 
+rewrite ! pattern_size_closed.
+cbv. auto. 
+eapply2 omega_k_closed.
+cbv; auto.
+discriminate .
+(* 5 *) 
+rewrite ! occurs_app.
+rewrite ! occurs_star_opt.
+rewrite ! occurs_app. 
+rewrite ! occurs_extension. 
+rewrite ! pattern_size_ab1. 
+rewrite ! pattern_size_app_comb2. 
+rewrite ! pattern_size_app_comb. 
+rewrite ! pattern_size_ref.
+rewrite ! pattern_size_closed.
+unfold app_comb; unfold_op. 
+rewrite ! occurs_app.
+unfold plus.
+rewrite ! occurs_op.
+rewrite ! occur_ref; unfold eqnat. omega. 
+eapply2 omega_k_closed. 
+eapply2 Y_k_closed.
+eapply2 A_k_closed. 
+cbv; auto. 
+eapply2 omega_k_closed.
+(* 4 *) 
+rewrite star_opt_occurs_true .
+discriminate. 
+rewrite ! occurs_app.
+rewrite ! occurs_star_opt.
+rewrite ! occurs_case. 
+rewrite ! pattern_size_app_comb. 
+rewrite ! pattern_size_ref.
+rewrite ! pattern_size_closed.
+cbv; auto. 
+eapply2 omega_k_closed. 
+cbv; auto. 
+discriminate.
+(* 3 *) 
+rewrite ! occurs_app.
+rewrite ! occurs_star_opt.
+rewrite ! occurs_case. 
+rewrite ! pattern_size_app_comb. 
+rewrite ! pattern_size_ref.
+rewrite ! pattern_size_closed.
+unfold plus. fold plus.
+rewrite ! occurs_app.
+rewrite! occur_ref. unfold eqnat.
+rewrite ! occurs_op. unfold plus. 
+omega. 
+eapply2 omega_k_closed. 
+cbv; auto.
+(* 2 *)  
+rewrite star_opt_occurs_true .
+discriminate. 
+rewrite ! occurs_app.
+rewrite ! occurs_extension.
+rewrite ! pattern_size_ab1. 
+rewrite ! pattern_size_app_comb2. 
+rewrite ! pattern_size_app_comb. 
+rewrite ! pattern_size_ref.
+rewrite ! pattern_size_closed.
+unfold app_comb; unfold_op. 
+rewrite ! occurs_app.
+rewrite ! occurs_op.
+rewrite ! occur_ref. unfold eqnat, plus . omega.
+eapply2 omega_k_closed. 
+eapply2 Y_k_closed.
+eapply2 A_k_closed. 
+cbv; auto. 
+eapply2 omega_k_closed.
+discriminate . 
+Qed. 
+
+
+Lemma subst_rec_preserves_sf_red1:
+forall M N P k, sf_red1 M N -> sf_red1 (subst_rec M P k) (subst_rec N P k).
+Proof. intros.  induction H; simpl; auto. Qed. 
+
+Lemma  subst_rec_preserves_multi_step: 
+forall (red: Tree -> Tree -> Prop), 
+(forall  M N P k, red M N -> red (subst_rec M P k) (subst_rec N P k)) -> 
+forall M N P k, multi_step red M N -> multi_step red  (subst_rec M P k) (subst_rec N P k).
+Proof.
+intros.  induction H0; auto.
+eapply succ_red. eapply2 H. eapply2 IHmulti_step. 
+Qed. 
+   
+
+Lemma  subst_rec_preserves_sf_red:
+forall M N, sf_red M N -> forall P k, sf_red (subst_rec M P k) (subst_rec N P k).
+Proof. intros. eapply2 subst_rec_preserves_multi_step. eapply2 subst_rec_preserves_sf_red1. Qed.
+ 
+
+Lemma subst_rec_preserves_ab_op: 
+forall M N k, subst_rec (ab_op M) N k = ab_op (subst_rec M N (S (S k))).
+Proof.
+intros. unfold ab_op. 
+rewrite ! subst_rec_preserves_star_opt.
+rewrite ! subst_rec_preserves_app_comb2.
+rewrite ! subst_rec_preserves_app_comb.
+rewrite subst_rec_closed. 
+2: rewrite A_k_closed; omega. 
+rewrite ! subst_rec_ref. insert_Ref_out.
+auto. 
+Qed. 
+ 
+
+Lemma b_a1_red: 
+forall M N P, sf_red (App (App (App b_op M) N) (App abs_op P)) 
+                     (App (App (App (App b_op M) N) abs_op) (App (App (App b_op M) N) P)).
+Proof.
+intros; unfold b_op. 
+eapply transitive_red. 
+eapply preserves_app_sf_red.
+eapply preserves_app_sf_red.
+eapply2 app_comb_red. auto.
+unfold abs_op. apply a1_aux.
+rewrite maxvar_ab_fn. rewrite b_op_closed. auto.  
+eapply transitive_red.    
+eapply2 Y2_fix.
+unfold b_fn at 1. 
+eapply transitive_red.
+eapply preserves_app_sf_red. 
+eapply2 star_opt_beta3. auto. 
+unfold subst.
+rewrite ! subst_rec_preserves_extension.
+(* 1 *) 
+eapply transitive_red.
+eapply2 extensions_by_matchfail.
+eapply2 matchfail_compound_l. 
+eapply2 matchfail_compound_r. 
+eapply2 matchfail_compound_r.
+unfold_op. 
+eapply2 matchfail_compound_l. 
+eapply2 matchfail_compound_r.
+eapply2 matchfail_compound_r.
+eapply2 matchfail_op.
+right. auto. discriminate .
+(* 1 *) 
+eapply transitive_red.
+eapply2 extensions_by_matchfail.
+eapply2 matchfail_compound_l. 
+eapply2 matchfail_compound_r. 
+eapply2 matchfail_compound_r.
+unfold_op. 
+eapply2 matchfail_compound_l. 
+eapply2 matchfail_compound_r.
+eapply2 matchfail_compound_r.
+eapply2 matchfail_op.
+right. auto. discriminate .
+(* 1 *) 
+eapply transitive_red.
+eapply2 extensions_by_matchfail.
+eapply2 matchfail_compound_l. 
+eapply2 matchfail_compound_r. 
+eapply2 matchfail_compound_r.
+unfold_op. 
+eapply2 matchfail_compound_l. 
+eapply2 matchfail_compound_r.
+eapply2 matchfail_compound_r.
+eapply2 matchfail_op.
+right. auto. discriminate .
+(* 1 *) 
+eapply transitive_red.
+eapply2 extensions_by_matchfail.
+eapply2 matchfail_compound_l. 
+eapply2 matchfail_compound_r. 
+eapply2 matchfail_compound_r.
+unfold_op. 
+eapply2 matchfail_compound_l. 
+eapply2 matchfail_compound_r.
+eapply2 matchfail_compound_r.
+eapply2 matchfail_op.
+right. auto. discriminate .
+(* 1 *) 
+eapply transitive_red.
+eapply2 extensions_by_matchfail.
+eapply2 matchfail_compound_l. 
+eapply2 matchfail_compound_r. 
+eapply2 matchfail_compound_r.
+unfold_op. 
+eapply2 matchfail_compound_l. 
+eapply2 matchfail_compound_r.
+eapply2 matchfail_compound_r.
+eapply2 matchfail_op.
+right. auto. discriminate .
+(* 1 *) 
+eapply transitive_red.
+eapply2 extensions_by_matching.
+unfold ab1. unfold_op. 
+eapply2 match_app.  
+eapply2 match_app.  
+eapply2 match_app.  
+eapply2 match_app.  
+eapply2 match_app.  
+eapply2 match_app.  
+eapply2 match_app.
+eapply2 program_matching.
+split; auto.
+repeat eapply2 nf_compound. 
+repeat eapply2 match_app.
+(* 3 *)   
+eapply2 match_app.  
+eapply2 match_app.  
+eapply2 match_app.  
+eapply2 match_app.  
+eapply2 match_app.  
+repeat eapply2 match_app.  
+eapply2 match_app.
+repeat eapply2 match_app. 
+eapply2 match_app.  
+eapply2 match_app.  
+repeat eapply2 match_app.  
+eapply2 match_app.  
+eapply2 match_app.  
+eapply2 match_app.
+eapply2 program_matching. 
+split; auto. 
+eapply2 program_matching. 
+split; auto. 
+eapply2 star_opt_normal.
+repeat eapply2 nf_compound. 
+(* 1 *) 
+unfold length; fold length. 
+rewrite ! map_lift0.
+rewrite ! app_nil_r. 
+unfold map. rewrite ! app_nil_l. 
+rewrite ! subst_rec_app.
+rewrite ! subst_rec_preserves_ab_op.
+rewrite ! pattern_size_ab1. 
+rewrite ! pattern_size_ref.
+rewrite ! subst_rec_ref. insert_Ref_out. 
+rewrite ! subst_rec_ref. insert_Ref_out. 
+rewrite ! subst_rec_ref. insert_Ref_out. 
+unfold plus, lift.
+rewrite ! lift_rec_lift_rec; try omega. unfold plus.   
+rewrite ! subst_rec_lift_rec; try omega.
+unfold app, fold_left.
+unfold subst. 
+rewrite ! subst_rec_app.
+rewrite ! subst_rec_preserves_ab_op. 
+rewrite ! subst_rec_ref. insert_Ref_out. 
+rewrite ! subst_rec_ref. insert_Ref_out. 
+rewrite ! subst_rec_lift_rec; try omega.
+unfold lift; rewrite ! lift_rec_null.
+rewrite lift_rec_lift_rec; try omega. unfold plus.  
+rewrite ! subst_rec_lift_rec; try omega.
+rewrite lift_rec_closed. 
+unfold abs_op. auto.
+rewrite maxvar_ab_fn. rewrite b_op_closed; auto. 
+Qed.
+
+
+Lemma b_b1_red: 
+forall M N P, sf_red (App (App (App b_op M) N) (App b_op P)) 
+     (App (App (App (App b_op M) N) b_op) (App (App (App b_op M) N) P)).
+Proof.
+intros; unfold b_op. 
+eapply transitive_red. 
+eapply preserves_app_sf_red.
+eapply preserves_app_sf_red.
+eapply2 app_comb_red. all: auto. 
+eapply transitive_red.    
+eapply2 Y2_fix.
+unfold b_fn at 1. 
+eapply transitive_red.
+eapply preserves_app_sf_red. 
+eapply2 star_opt_beta3. auto. 
+unfold subst.
+rewrite ! subst_rec_preserves_extension.
+(* 1 *) 
+eapply transitive_red. 
+eapply preserves_app_sf_red. auto.  
+unfold h_op. 
+eapply transitive_red. 
+eapply transitive_red. 
+eapply app_comb_red.
+eapply preserves_app_sf_red. 
+eapply app_comb_red.  auto.
+eapply transitive_red.
+eapply preserves_app_sf_red. 
+eapply preserves_app_sf_red. 
+eapply app_comb_red.  auto. auto. 
+eapply transitive_red.
+eapply preserves_app_sf_red. 
+eapply preserves_app_sf_red. 
+unfold A_k.
+eapply2 star_opt_beta2. auto. auto. 
+unfold subst. 
+rewrite ! subst_rec_preserves_app_comb. 
+rewrite ! subst_rec_ref. insert_Ref_out.  
+rewrite ! subst_rec_ref. insert_Ref_out.  
+unfold lift; rewrite ! lift_rec_null.
+rewrite ! lift_rec_closed. 
+2: eapply2 omega_k_closed. 
+eapply transitive_red. 
+eapply preserves_app_sf_red.
+eapply2 app_comb_red. auto. 
+rewrite (subst_rec_closed (omega_k 2)) at 1.
+2: rewrite omega_k_closed; omega.
+match goal with 
+| |- multi_step sf_red1 (App (App (App (subst_rec (subst_rec ?M ?N1 0) ?N2 0) ?P1) ?P2) ?P3) _ => 
+replace (App (App (subst_rec (subst_rec M N1 0) N2 0) P1) P2) with 
+(subst_rec (subst_rec (App (App M P1) P2) N1 0) N2 0) 
+end.
+eapply preserves_app_sf_red. 
+eapply subst_rec_preserves_sf_red.
+eapply subst_rec_preserves_sf_red.
+eapply2 star_opt_beta2.  auto. 
+rewrite ! subst_rec_app. 
+rewrite (subst_rec_closed b_fn) at 1.
+rewrite (subst_rec_closed b_fn) at 1.
+rewrite (subst_rec_closed (app_comb (omega_k 2) (omega_k 2))) at 1. 
+rewrite (subst_rec_closed (app_comb (omega_k 2) (omega_k 2))) at 1.
+auto. 
+3, 4: rewrite b_fn_closed; auto. 
+1,2: unfold app_comb; unfold_op;  rewrite ! maxvar_app; rewrite ! omega_k_closed; cbv; auto.
+(* 1 *)      
+eapply transitive_red.
+eapply preserves_app_sf_red.
+auto. 
+unfold subst; rewrite ! subst_rec_preserves_app_comb.
+rewrite (subst_rec_closed (star_opt _)) at 1. 2: cbv; auto. 
+rewrite (subst_rec_closed (star_opt _)) at 1. 2: cbv; auto. 
+rewrite (subst_rec_closed (star_opt _)) at 1. 2: cbv; auto. 
+rewrite (subst_rec_closed (star_opt _)) at 1. 2: cbv; auto. 
+rewrite subst_rec_ref at 1. insert_Ref_out. 
+rewrite subst_rec_ref at 1. insert_Ref_out. 
+rewrite subst_rec_ref at 1. insert_Ref_out. 
+unfold lift; rewrite ! lift_rec_null. 
+rewrite subst_rec_lift_rec; try omega. 
+rewrite lift_rec_null. 
+rewrite ! subst_rec_closed. 
+2: rewrite b_fn_closed; auto. 
+2: rewrite subst_rec_closed. 
+2: rewrite b_fn_closed; auto. 
+2: rewrite b_fn_closed; auto. 
+2: rewrite maxvar_app_comb; rewrite ! omega_k_closed; auto. 
+2: rewrite subst_rec_closed.  2, 3: rewrite maxvar_app_comb.
+2,3: rewrite omega_k_closed; auto.
+eapply transitive_red. eapply2 app_comb_red. 
+eapply2 star_opt_beta2.
+(* 1 *)  
+eapply transitive_red. 
+eapply extensions_by_matchfail.
+unfold subst; rewrite ! subst_rec_preserves_app_comb.
+rewrite ! subst_rec_ref. insert_Ref_out. 
+rewrite ! subst_rec_ref. insert_Ref_out. 
+unfold lift; rewrite ! lift_rec_null. 
+rewrite subst_rec_lift_rec; try omega. 
+rewrite lift_rec_null.
+rewrite ! (subst_rec_closed a_op).
+2: cbv; auto. 
+eapply2 matchfail_app_comb_l.
+eapply2 matchfail_compound_l. 
+fold star_opt. 
+eapply2 matchfail_compound_r.  
+eapply2 matchfail_compound_r.  
+unfold_op; unfold occurs. unfold plus. 
+eapply2 matchfail_compound_l. 
+unfold_op; auto.
+unfold_op; eapply2 matchfail_compound_r.
+(* 1 *)  
+eapply transitive_red. 
+eapply preserves_app_sf_red. auto. 
+unfold subst; rewrite ! subst_rec_preserves_app_comb.
+rewrite ! subst_rec_ref. insert_Ref_out. 
+rewrite ! subst_rec_ref. insert_Ref_out. 
+unfold lift; rewrite ! lift_rec_null. 
+rewrite subst_rec_lift_rec; try omega. 
+rewrite lift_rec_null.
+rewrite ! (subst_rec_closed a_op).
+2: cbv; auto. auto. 
+(* 1 *)  
+eapply transitive_red. 
+eapply extensions_by_matchfail.
+eapply2 matchfail_app_comb_l.
+eapply2 matchfail_compound_l. 
+fold star_opt. 
+eapply2 matchfail_compound_r.  
+eapply2 matchfail_compound_r.  
+unfold_op; unfold occurs. 
+unfold plus. 
+cbv. 
+eapply2 matchfail_compound_l. 
+(* 1 *)  
+eapply transitive_red. 
+eapply extensions_by_matchfail.
+eapply2 matchfail_app_comb_l.
+eapply2 matchfail_compound_l. 
+fold star_opt. 
+eapply2 matchfail_compound_r.  
+eapply2 matchfail_compound_r.  
+unfold_op; unfold occurs. 
+unfold plus. cbv. 
+eapply2 matchfail_compound_l.
+(* 1 *)  
+eapply transitive_red. 
+eapply extensions_by_matchfail.
+eapply2 matchfail_app_comb_l.
+eapply2 matchfail_compound_l. 
+fold star_opt. 
+eapply2 matchfail_compound_r.  
+eapply2 matchfail_compound_r.  
+unfold_op; unfold occurs. 
+unfold plus. 
+cbv. 
+eapply2 matchfail_compound_l. 
+(* 1 *)  
+eapply transitive_red. 
+eapply extensions_by_matchfail.
+eapply2 matchfail_app_comb_r.
+eapply2 matchfail_app_comb_l.
+eapply2 matchfail_app_comb_l.
+unfold A_k. 
+unfold app_comb. unfold_op.
+rewrite star_opt_occurs_true.
+rewrite star_opt_occurs_true.
+eapply2 matchfail_compound_l.  
+eapply2 matchfail_compound_r.  
+eapply2 matchfail_compound_r.
+eapply2 matchfail_compound_l.  
+unfold_op; auto.
+eapply2 matchfail_compound_r.  
+unfold_op; auto.
+unfold_op; eapply2 matchfail_op. 
+right; auto.
+discriminate.
+rewrite! occurs_app. 
+rewrite ! occurs_star_opt.
+rewrite! occurs_app. 
+rewrite ! occur_ref.
+rewrite ! occurs_op; unfold eqnat. unfold plus; fold plus. 
+omega. 
+discriminate.
+rewrite! occurs_app. 
+rewrite ! occur_ref.
+rewrite ! occurs_op; unfold eqnat. unfold plus; fold plus. 
+omega. 
+discriminate.
+(* 1 *) 
+eapply transitive_red. 
+eapply extensions_by_matchfail.
+eapply2 matchfail_compound_l. 
+eapply2 matchfail_compound_r. 
+eapply2 matchfail_compound_r. 
+eapply2 matchfail_compound_l. 
+unfold_op. 
+eapply2 matchfail_compound_r.
+(* 1 *) 
+eapply transitive_red. 
+eapply2 extensions_by_matching.
+unfold app_comb; unfold_op. 
+eapply2 match_app.
+repeat eapply2 match_app. 
+eapply2 match_app.
+eapply2 match_app.
+eapply2 match_app.
+eapply2 match_app.
+eapply2 match_app.
+eapply2 match_app.
+eapply2 match_app.
+eapply2 match_app.
+eapply2 match_app.
+eapply2 match_app.
+eapply2 match_app.
+eapply2 match_app.
+eapply2 match_app.
+eapply2 match_app.
+eapply2 match_app.
+eapply2 match_app.
+eapply2 match_app.
+eapply2 match_app.
+eapply2 match_app.
+eapply2 match_app.
+eapply2 match_app.
+eapply2 match_app.
+eapply2 match_app.
+eapply2 match_app.
+eapply2 match_app.
+eapply2 match_app.
+eapply2 match_app.
+eapply2 match_app.
+eapply2 program_matching.
+split.  eapply2 omega_k_normal. eapply2 omega_k_closed.  
+eapply2 match_app.
+eapply2 program_matching.
+split.  eapply2 omega_k_normal. eapply2 omega_k_closed.  
+eapply2 program_matching.
+split.  eapply2 nf_compound.
+repeat eapply2 star_opt_normal. 
+repeat eapply2 nf_compound. 
+cbv. auto. 
+(* 1 *) 
+unfold length; fold length. 
+rewrite ! map_lift0.
+rewrite ! app_nil_r. 
+unfold map. rewrite ! app_nil_l. 
+rewrite ! subst_rec_app.
+rewrite ! subst_rec_preserves_app_comb.
+rewrite (subst_rec_closed (A_k _)) at 1. 
+rewrite (subst_rec_closed (A_k _)) at 1. 
+rewrite (subst_rec_closed (A_k _)) at 1. 
+rewrite (subst_rec_closed (omega_k _)) at 1. 
+rewrite (subst_rec_closed (omega_k _)) at 1. 
+rewrite (subst_rec_closed (omega_k _)) at 1. 
+rewrite (subst_rec_closed (omega_k _)) at 1. 
+rewrite (subst_rec_closed (omega_k _)) at 1. 
+rewrite (subst_rec_closed (omega_k _)) at 1. 
+rewrite ! pattern_size_app_comb. 
+rewrite ! pattern_size_ref.
+rewrite ! pattern_size_closed.
+2: cbv; auto. 2: eapply2 omega_k_closed. 
+all: try (rewrite omega_k_closed; omega). 
+all: try (rewrite A_k_closed; omega).
+(* 1 *)  
+rewrite ! subst_rec_ref. insert_Ref_out. 
+rewrite ! subst_rec_ref. insert_Ref_out. 
+rewrite ! subst_rec_ref. insert_Ref_out. 
+unfold plus, lift.
+unfold app, fold_left.
+unfold subst. 
+rewrite ! subst_rec_app.
+rewrite ! subst_rec_preserves_app_comb. 
+rewrite (subst_rec_closed (A_k _)). 
+rewrite (subst_rec_closed (A_k _)). 
+rewrite (subst_rec_closed (omega_k _)) at 1. 
+rewrite (subst_rec_closed (omega_k _)) at 1. 
+rewrite (subst_rec_closed (omega_k _)) at 1. 
+rewrite (subst_rec_closed (omega_k _)) at 1. 
+all: try (rewrite omega_k_closed; omega).
+all: try (rewrite A_k_closed; omega).
+rewrite ! subst_rec_ref. insert_Ref_out. 
+rewrite ! subst_rec_ref. insert_Ref_out. 
+unfold lift; rewrite ! lift_rec_null.
+rewrite ! lift_rec_lift_rec; try omega. unfold plus. 
+rewrite ! subst_rec_lift_rec; try omega.
+rewrite ! lift_rec_null. 
+auto.
+Qed. 
+
+
+
+Lemma b_h1_red: 
+forall M N P, sf_red (App (App (App b_op M) N) (App h_op P)) 
+(App (App (App (App b_op M) N) h_op) (App (App (App b_op M) N) P)).
+Proof.
+intros; unfold b_op. 
+eapply transitive_red. 
+eapply preserves_app_sf_red.
+eapply preserves_app_sf_red.
+eapply2 app_comb_red. all: auto. 
+eapply transitive_red.    
+eapply2 Y2_fix.
+unfold b_fn at 1. 
+eapply transitive_red.
+eapply preserves_app_sf_red. 
+eapply2 star_opt_beta3. auto. 
+unfold subst.
+rewrite ! subst_rec_preserves_extension.
+(* 1 *) 
+eapply transitive_red. 
+eapply preserves_app_sf_red. auto.  
+unfold h_op. 
+eapply transitive_red. 
+eapply transitive_red. 
+eapply app_comb_red.
+eapply preserves_app_sf_red. 
+eapply app_comb_red.  auto.
+eapply transitive_red.
+eapply preserves_app_sf_red. 
+eapply preserves_app_sf_red. 
+eapply app_comb_red.  auto. auto. 
+eapply transitive_red.
+eapply preserves_app_sf_red. 
+eapply preserves_app_sf_red. 
+unfold A_k.
+eapply2 star_opt_beta2. auto. auto. 
+unfold subst. 
+rewrite ! subst_rec_preserves_app_comb. 
+rewrite ! subst_rec_ref. insert_Ref_out.  
+rewrite ! subst_rec_ref. insert_Ref_out.  
+unfold lift; rewrite ! lift_rec_null.
+rewrite ! lift_rec_closed. 
+2: eapply2 omega_k_closed. 
+eapply transitive_red. 
+eapply preserves_app_sf_red.
+eapply2 app_comb_red. auto. 
+rewrite (subst_rec_closed (omega_k 2)) at 1.
+2: rewrite omega_k_closed; omega.
+match goal with 
+| |- multi_step sf_red1 (App (App (App (subst_rec (subst_rec ?M ?N1 0) ?N2 0) ?P1) ?P2) ?P3) _ => 
+replace (App (App (subst_rec (subst_rec M N1 0) N2 0) P1) P2) with 
+(subst_rec (subst_rec (App (App M P1) P2) N1 0) N2 0) 
+end.
+eapply preserves_app_sf_red. 
+eapply subst_rec_preserves_sf_red.
+eapply subst_rec_preserves_sf_red.
+eapply2 star_opt_beta2.  auto. 
+rewrite ! subst_rec_app.
+rewrite (subst_rec_closed h_fn) at 1.
+rewrite (subst_rec_closed h_fn) at 1.
+rewrite (subst_rec_closed (app_comb (omega_k 2) (omega_k 2))) at 1. 
+rewrite (subst_rec_closed (app_comb (omega_k 2) (omega_k 2))) at 1.
+auto. 
+3, 4: cbv; auto. 
+1,2: unfold app_comb; unfold_op;  rewrite ! maxvar_app; rewrite ! omega_k_closed; cbv; auto.
+(* 1 *)      
+eapply transitive_red.
+eapply preserves_app_sf_red.
+auto. 
+unfold subst; rewrite ! subst_rec_preserves_app_comb.
+rewrite (subst_rec_closed (star_opt _)) at 1. 2: cbv; auto. 
+rewrite (subst_rec_closed (star_opt _)) at 1. 2: cbv; auto. 
+rewrite (subst_rec_closed (star_opt _)) at 1. 2: cbv; auto. 
+rewrite (subst_rec_closed (star_opt _)) at 1. 2: cbv; auto. 
+rewrite subst_rec_ref at 1. insert_Ref_out. 
+rewrite subst_rec_ref at 1. insert_Ref_out. 
+rewrite subst_rec_ref at 1. insert_Ref_out. 
+unfold lift; rewrite ! lift_rec_null. 
+rewrite subst_rec_lift_rec; try omega. 
+rewrite lift_rec_null. 
+rewrite ! subst_rec_closed. 
+2: cbv; auto. 
+2: rewrite subst_rec_closed. 
+2: cbv; auto. 
+2: cbv; auto. 
+2: rewrite maxvar_app_comb; rewrite ! omega_k_closed; auto. 
+2: rewrite subst_rec_closed.  2, 3: rewrite maxvar_app_comb.
+2,3: rewrite omega_k_closed; auto.
+eapply transitive_red. eapply2 app_comb_red. 
+eapply2 star_opt_beta2.
+(* 1 *)  
+eapply transitive_red. 
+eapply extensions_by_matchfail.
+unfold subst; rewrite ! subst_rec_preserves_app_comb.
+rewrite ! subst_rec_ref. insert_Ref_out. 
+rewrite ! subst_rec_ref. insert_Ref_out. 
+unfold lift; rewrite ! lift_rec_null. 
+rewrite subst_rec_lift_rec; try omega. 
+rewrite lift_rec_null.
+rewrite ! (subst_rec_closed a_op).
+2: cbv; auto. 
+eapply2 matchfail_app_comb_l.
+eapply2 matchfail_compound_l. 
+fold star_opt. 
+eapply2 matchfail_compound_r.  
+eapply2 matchfail_compound_r.  
+unfold_op; unfold occurs. 
+unfold plus. cbv. 
+eapply2 matchfail_compound_l. 
+(* 1 *)  
+eapply transitive_red. 
+eapply preserves_app_sf_red. auto. 
+unfold subst; rewrite ! subst_rec_preserves_app_comb.
+rewrite ! subst_rec_ref. insert_Ref_out. 
+rewrite ! subst_rec_ref. insert_Ref_out. 
+unfold lift; rewrite ! lift_rec_null. 
+rewrite subst_rec_lift_rec; try omega. 
+rewrite lift_rec_null.
+rewrite ! (subst_rec_closed a_op).
+2: cbv; auto. auto. 
+(* 1 *)  
+eapply transitive_red. 
+eapply extensions_by_matchfail.
+eapply2 matchfail_app_comb_l.
+eapply2 matchfail_compound_l. 
+fold star_opt. 
+eapply2 matchfail_compound_r.  
+eapply2 matchfail_compound_r.  
+unfold_op; unfold occurs. 
+unfold plus. 
+cbv. 
+eapply2 matchfail_compound_l. 
+(* 1 *)  
+eapply transitive_red. 
+eapply extensions_by_matchfail.
+eapply2 matchfail_app_comb_l.
+eapply2 matchfail_compound_l. 
+fold star_opt. 
+eapply2 matchfail_compound_r.  
+eapply2 matchfail_compound_r.  
+unfold_op; unfold occurs. 
+unfold plus. cbv. 
+eapply2 matchfail_compound_l.
+(* 1 *)  
+eapply transitive_red. 
+eapply extensions_by_matchfail.
+eapply2 matchfail_app_comb_l.
+eapply2 matchfail_compound_l. 
+fold star_opt. 
+eapply2 matchfail_compound_r.  
+eapply2 matchfail_compound_r.  
+unfold_op; unfold occurs. 
+unfold plus.
+cbv. 
+eapply2 matchfail_compound_l. 
+(* 1 *)  
+eapply transitive_red. 
+eapply extensions_by_matchfail.
+eapply2 matchfail_app_comb_r.
+eapply2 matchfail_app_comb_l.
+eapply2 matchfail_app_comb_l.
+unfold A_k. 
+unfold app_comb. unfold_op.
+rewrite star_opt_occurs_true.
+rewrite star_opt_occurs_true.
+eapply2 matchfail_compound_l.  
+eapply2 matchfail_compound_r.  
+eapply2 matchfail_compound_r.
+cbv.
+eapply2 matchfail_compound_l.  
+eapply2 matchfail_compound_r.  
+eapply2 matchfail_op.
+right; auto. discriminate.
+rewrite ! occurs_app.
+rewrite occurs_star_opt.
+rewrite ! occurs_app.
+rewrite ! occur_ref.
+unfold eqnat.
+omega.
+discriminate.
+rewrite ! occurs_app.
+rewrite ! occur_ref.
+unfold eqnat.
+omega.
+discriminate.
+(* 1 *) 
+eapply transitive_red. 
+eapply extensions_by_matchfail.
+eapply2 matchfail_compound_l. 
+eapply2 matchfail_compound_r. 
+eapply2 matchfail_compound_r. 
+eapply2 matchfail_compound_l. 
+unfold_op. 
+eapply2 matchfail_compound_r.
+(* 1 *) 
+eapply transitive_red. 
+eapply2 extensions_by_matching.
+unfold app_comb; unfold_op. 
+eapply2 match_app.
+repeat eapply2 match_app. 
+eapply2 match_app.
+eapply2 match_app.
+eapply2 match_app.
+eapply2 match_app.
+eapply2 match_app.
+eapply2 match_app.
+eapply2 match_app.
+eapply2 match_app.
+eapply2 match_app.
+eapply2 match_app.
+eapply2 match_app.
+eapply2 match_app.
+eapply2 match_app.
+eapply2 match_app.
+eapply2 match_app.
+eapply2 match_app.
+eapply2 match_app.
+eapply2 match_app.
+eapply2 match_app.
+eapply2 match_app.
+eapply2 match_app.
+eapply2 match_app.
+eapply2 match_app.
+eapply2 match_app.
+eapply2 match_app.
+eapply2 match_app.
+eapply2 match_app.
+eapply2 match_app.
+eapply2 program_matching.
+split.  eapply2 omega_k_normal. eapply2 omega_k_closed.  
+eapply2 match_app.
+eapply2 program_matching.
+split.  eapply2 omega_k_normal. eapply2 omega_k_closed.  
+eapply2 program_matching.
+split.  eapply2 nf_compound.
+repeat eapply2 star_opt_normal. 
+repeat eapply2 nf_compound. 
+cbv. auto. 
+(* 1 *) 
+unfold length; fold length. 
+rewrite ! map_lift0.
+rewrite ! app_nil_r. 
+unfold map. rewrite ! app_nil_l. 
+rewrite ! subst_rec_app.
+rewrite ! subst_rec_preserves_app_comb.
+rewrite (subst_rec_closed (A_k _)) at 1. 
+rewrite (subst_rec_closed (A_k _)) at 1. 
+rewrite (subst_rec_closed (A_k _)) at 1. 
+rewrite (subst_rec_closed (omega_k _)) at 1. 
+rewrite (subst_rec_closed (omega_k _)) at 1. 
+rewrite (subst_rec_closed (omega_k _)) at 1. 
+rewrite (subst_rec_closed (omega_k _)) at 1. 
+rewrite (subst_rec_closed (omega_k _)) at 1. 
+rewrite (subst_rec_closed (omega_k _)) at 1. 
+rewrite ! pattern_size_app_comb. 
+rewrite ! pattern_size_ref.
+rewrite ! pattern_size_closed.
+2: cbv; auto. 2: eapply2 omega_k_closed. 
+all: try (rewrite omega_k_closed; omega). 
+all: try (rewrite A_k_closed; omega).
+(* 1 *)  
+rewrite ! subst_rec_ref. insert_Ref_out. 
+rewrite ! subst_rec_ref. insert_Ref_out. 
+rewrite ! subst_rec_ref. insert_Ref_out. 
+unfold plus, lift.
+unfold app, fold_left.
+unfold subst. 
+rewrite ! subst_rec_app.
+rewrite ! subst_rec_preserves_app_comb. 
+rewrite (subst_rec_closed (A_k _)). 
+rewrite (subst_rec_closed (A_k _)). 
+rewrite (subst_rec_closed (omega_k _)) at 1. 
+rewrite (subst_rec_closed (omega_k _)) at 1. 
+rewrite (subst_rec_closed (omega_k _)) at 1. 
+rewrite (subst_rec_closed (omega_k _)) at 1. 
+all: try (rewrite omega_k_closed; omega).
+all: try (rewrite A_k_closed; omega).
+rewrite ! subst_rec_ref. insert_Ref_out. 
+rewrite ! subst_rec_ref. insert_Ref_out. 
+unfold lift; rewrite ! lift_rec_null.
+rewrite ! lift_rec_lift_rec; try omega. unfold plus. 
+rewrite ! subst_rec_lift_rec; try omega.
+rewrite ! lift_rec_null.
+auto.
+Qed. 
